Stutter.v
@@ -1,0 +1,475 @@
+Require Import MyTactics.
+Require Export List.
+Require Import RelationClasses.
+
+Inductive stutter_equiv {A} : list A -> list A -> Prop :=
+| stutter_nil: stutter_equiv nil nil
+| stutter_same:
+    forall a l1 l2,
+      stutter_equiv l1 l2 ->
+      stutter_equiv (a :: l1) (a :: l2)
+| stutter_left:
+    forall a l1 l2,
+      stutter_equiv (a :: l1) l2 ->
+      stutter_equiv (a :: a :: l1) l2
+| stutter_right:
+    forall a l1 l2,
+      stutter_equiv l1 (a :: l2) ->
+      stutter_equiv l1 (a :: a :: l2)
+.
+Hint Constructors stutter_equiv.
+
+Lemma stutter_equiv_refl {A} :
+  forall (l : list A),
+    stutter_equiv l l.
+Proof.
+intros x. induction x; auto.
+Qed.
+
+Hint Extern 3 (stutter_equiv _ _) => reflexivity.
+
+Lemma stutter_equiv_sym {A} :
+  forall (l1 l2 : list A),
+    stutter_equiv l1 l2 ->
+    stutter_equiv l2 l1.
+Proof.
+intros x y Hxy. induction Hxy; auto.
+Qed.
+
+Lemma stutter_equiv_cons_inv {A} :
+  forall a1 a2 (l1 l2 : list A),
+    stutter_equiv (a1 :: l1) (a2 :: l2) ->
+    a1 = a2.
+Proof.
+intros a1 a2 l1 l2 H.
+remember (a1 :: l1) as l1'.
+remember (a2 :: l2) as l2'.
+generalize dependent l2. generalize dependent l1.
+revert a2. revert a1.
+rename l1' into l1. rename l2' into l2.
+induction H; intros a1' a2' l1' H1' l2' H2'; inversion H1'; subst; eauto.
+* inversion H2'; subst; eauto.
+* inversion H2'; subst; eauto.
+Qed.
+
+Lemma stutter_equiv_cons_left_inv {A} :
+  forall a (l1 l2: list A),
+    stutter_equiv (a :: l1) l2 ->
+    exists l2', l2 = a :: l2'.
+Proof.
+intros a l1 l2 H.
+remember (a :: l1) as l1'.
+generalize dependent l1. revert a.
+rename l1' into l1.
+induction H; intros a' l' Heq; inversion Heq; subst; eauto.
+apply stutter_equiv_cons_inv in H. subst. eauto.
+Qed.
+
+Lemma stutter_equiv_cons_right_inv {A} :
+  forall a (l1 l2: list A),
+    stutter_equiv l1 (a :: l2) ->
+    exists l1', l1 = a :: l1'.
+Proof.
+intros a l1 l2 H.
+apply stutter_equiv_sym in H.
+eapply stutter_equiv_cons_left_inv. eauto.
+Qed.
+
+Lemma stutter_equiv_cons_right_add_left {A} :
+  forall a (l1 l2: list A),
+    stutter_equiv l1 (a :: l2) ->
+    stutter_equiv (a :: l1) (a :: l2).
+Proof.
+intros a l1 l2 H.
+destruct (stutter_equiv_cons_right_inv _ _ _ H) as [l1' H'].
+subst. auto.
+Qed.
+
+Lemma stutter_equiv_cons_left_add_right {A} :
+  forall a (l1 l2: list A),
+    stutter_equiv (a :: l1) l2 ->
+    stutter_equiv (a :: l1) (a :: l2).
+Proof.
+intros a l1 l2 H.
+destruct (stutter_equiv_cons_left_inv _ _ _ H) as [l2' H'].
+subst. auto.
+Qed.
+
+Lemma stutter_equiv_nil_left_inv {A} :
+  forall (l: list A),
+    stutter_equiv nil l ->
+    l = nil.
+Proof.
+intros l2 H12. remember nil as l1.
+induction H12; try congruence.
+specialize (IHstutter_equiv Heql1). congruence.
+Qed.
+
+Lemma stutter_equiv_nil_right_inv {A} :
+  forall (l: list A),
+    stutter_equiv l nil ->
+    l = nil.
+Proof.
+intros l H. apply stutter_equiv_nil_left_inv.
+apply stutter_equiv_sym. assumption.
+Qed.
+
+Lemma stutter_equiv_cons_end_inv {A} :
+  forall a1 a2 (l1 l2 : list A),
+    stutter_equiv (l1 ++ a1 :: nil) (l2 ++ a2 :: nil) ->
+    a1 = a2.
+Proof.
+intros a1 a2 l1 l2 H.
+remember (l1 ++ a1 :: nil) as l1'.
+remember (l2 ++ a2 :: nil) as l2'.
+generalize dependent l2. generalize dependent l1.
+revert a2. revert a1.
+rename l1' into l1. rename l2' into l2.
+induction H; intros a1' a2' l1' H1' l2' H2'; inversion H1'; subst.
+* exfalso. destruct l1'; simpl in H1'; congruence.
+* destruct l1' as [|a1'' l1']; destruct l2' as [|a2'' l2']; simpl in *.
+  - congruence.
+  - exfalso. inversion H1'; subst.
+    apply stutter_equiv_nil_left_inv in H. subst.
+    destruct l2'; simpl in H2'; congruence.
+  - exfalso. inversion H2'; subst.
+    apply stutter_equiv_nil_right_inv in H. subst.
+    destruct l1'; simpl in H1'; congruence.
+  - inversion H1'; subst. inversion H2'; subst. eauto.
+* destruct l1' as [| a1'' l1'].
+  - exfalso. inversion H1.
+  - rewrite <- app_comm_cons in H1. inversion H1; subst.
+    destruct l2' as [| a2'' l2'].
+    + apply stutter_equiv_cons_inv in H. subst. eauto.
+    + rewrite <- app_comm_cons in H.
+      apply stutter_equiv_cons_inv in H. subst.
+      eauto.
+* destruct l2' as [| a2'' l2'].
+  - exfalso. inversion H2'.
+  - rewrite <- app_comm_cons in H2'. inversion H2'; subst.
+    destruct l1' as [| a1'' l1'].
+    + apply stutter_equiv_cons_inv in H. subst. eauto.
+    + rewrite <- app_comm_cons in H.
+      apply stutter_equiv_cons_inv in H. subst.
+      eauto.
+Qed.
+
+Lemma stutter_equiv_cons_end_left_inv {A} :
+  forall a (l1 l2: list A),
+    stutter_equiv (l1 ++ a :: nil) l2 ->
+    exists l2', l2 = l2' ++ a :: nil.
+Proof.
+intros a l1 l2 H.
+remember (l1 ++ a :: nil) as l1'.
+generalize dependent l1. revert a.
+rename l1' into l1.
+induction H; intros a' l' Heq; eauto.
+* destruct l' as [| a'' l'].
+  - inversion Heq; subst.
+    apply stutter_equiv_nil_left_inv in H. subst. eauto.
+  - rewrite <- app_comm_cons in Heq. inversion Heq; subst.
+    destruct (IHstutter_equiv a' l' eq_refl) as [l0 Hl0].
+    subst.
+    exists (a'' :: l0). apply app_comm_cons.
+* destruct l' as [| a'' l'].
+  - exfalso. inversion Heq.
+  - rewrite <- app_comm_cons in Heq. inversion Heq; subst.
+    destruct (IHstutter_equiv a' l') as [l0 Hl0].
+    congruence. subst. eauto.
+* subst. destruct (IHstutter_equiv a' l' eq_refl) as [l0 Hl0].
+  exists (a :: l0). rewrite <- app_comm_cons. congruence.
+Qed.
+
+Lemma stutter_equiv_cons_end_right_inv {A} :
+  forall a (l1 l2: list A),
+    stutter_equiv l1 (l2 ++ a :: nil) ->
+    exists l1', l1 = l1' ++ a :: nil.
+Proof.
+intros a l1 l2 H.
+apply stutter_equiv_sym in H.
+eapply stutter_equiv_cons_end_left_inv. eauto.
+Qed.
+
+Lemma stutter_equiv_cons_end_right_add_left {A} :
+  forall a (l1 l2: list A),
+    stutter_equiv l1 (l2 ++ a :: nil) ->
+    stutter_equiv (l1 ++ a :: nil) (l2 ++ a :: nil).
+Proof.
+intros a l1 l2 H.
+remember (l2 ++ a :: nil) as l2'.
+generalize dependent l2. revert a.
+rename l2' into l2.
+induction H; intros a' l2' Heq.
+* exfalso. destruct l2'; simpl in Heq; congruence.
+* destruct l2' as [| a2'' l2'].
+  - inversion Heq; subst.
+    apply stutter_equiv_nil_right_inv in H. subst.
+    simpl. auto.
+  - rewrite <- app_comm_cons in Heq. inversion Heq; subst.
+    rewrite <- app_comm_cons. apply stutter_same.
+    eauto.
+* subst. rewrite <- app_comm_cons. rewrite <- app_comm_cons.
+  apply stutter_left. rewrite app_comm_cons. eauto.
+* destruct l2' as [|a2'' l2'].
+  - exfalso. inversion Heq.
+  - rewrite <- app_comm_cons in Heq. inversion Heq; subst.
+    apply stutter_right. eauto.
+Qed.
+
+Lemma stutter_equiv_cons_end_left_add_right {A} :
+  forall a (l1 l2: list A),
+    stutter_equiv (l1 ++ a :: nil) l2 ->
+    stutter_equiv (l1 ++ a :: nil) (l2 ++ a :: nil).
+Proof.
+intros a l1 l2 H.
+apply stutter_equiv_sym.
+apply stutter_equiv_cons_end_right_add_left.
+apply stutter_equiv_sym. trivial.
+Qed.
+
+Lemma stutter_equiv_trans_strong {A} :
+  forall n (l1 l2 l3: list A),
+    length l1 + length l2 + length l3 <= n ->
+    stutter_equiv l1 l2 ->
+    stutter_equiv l2 l3 ->
+    stutter_equiv l1 l3.
+Proof.
+intros n; induction n; intros l1 l2 l3 Hn H12 H23.
+* destruct l1; destruct l2; destruct l3; simpl in Hn; auto.
+* inversion H12; subst; simpl in Hn; auto.
+  - inversion H23; subst; simpl in Hn.
+    + apply stutter_same. apply (IHn l0 l4 l2); auto.
+    + apply (IHn (a :: l0) (a :: l1) l3);
+      auto using stutter_equiv_cons_right_add_left.
+    + apply stutter_right.
+      apply (IHn (a :: l0) (a :: l4) (a0 :: l2)); auto.
+  - apply stutter_left.
+    apply (IHn (a :: l0) l2 l3); auto.
+  - inversion H23; subst; simpl in Hn.
+    + apply (IHn l1 (a :: l4) (a :: l2));
+      auto using stutter_equiv_cons_left_add_right.
+    + apply (IHn l1 (a :: l4) l3); auto.
+    + apply stutter_right.
+      apply (IHn l1 (a :: a :: l4) (a0 :: l2)); auto.
+Qed.
+
+Lemma stutter_equiv_trans {A} :
+  forall (l1 l2 l3: list A),
+    stutter_equiv l1 l2 ->
+    stutter_equiv l2 l3 ->
+    stutter_equiv l1 l3.
+Proof.
+intros l1 l2 l3 H12 H23.
+apply (stutter_equiv_trans_strong (length l1 + length l2 + length l3) l1 l2 l3);
+trivial.
+Qed.
+
+Instance stutter_equiv_Equivalence {A} : Equivalence (@stutter_equiv A).
+Proof.
+constructor.
+* exact stutter_equiv_refl.
+* exact stutter_equiv_sym.
+* exact stutter_equiv_trans.
+Defined.
+
+Lemma stutter_equiv_in {A} :
+  forall (l1 l2 : list A),
+    stutter_equiv l1 l2 ->
+    forall a, In a l1 -> In a l2.
+Proof.
+intros l1 l2 H a Ha. induction H.
+* inversion Ha.
+* destruct Ha as [Ha | Ha].
+  - left; congruence.
+  - right; auto.
+* destruct Ha as [Ha | Ha].
+  - subst; apply IHstutter_equiv. left; trivial.
+  - destruct Ha as [Ha | Ha]; apply IHstutter_equiv.
+    + left; congruence.
+    + right; trivial.
+* right. auto.
+Qed.
+
+Lemma stutter_equiv_app_left {A} :
+  forall (l l1 l2: list A),
+    stutter_equiv l1 l2 ->
+    stutter_equiv (l ++ l1) (l ++ l2).
+Proof.
+intros l l1 l2 H. induction l; simpl; auto.
+Qed.
+
+Lemma stutter_equiv_app_right {A} :
+  forall (l l1 l2: list A),
+    stutter_equiv l1 l2 ->
+    stutter_equiv (l1 ++ l) (l2 ++ l).
+Proof.
+intros l. induction l; intros l1 l2 H.
+* repeat rewrite app_nil_r. assumption.
+* replace (a :: l) with ((a :: nil) ++ l) by reflexivity.
+  repeat rewrite app_assoc. apply IHl.
+  clear IHl l. induction H; simpl; auto.
+Qed.
+
+Lemma stutter_equiv_congruence {A} :
+  forall (l1 l2 l3 l4: list A),
+    stutter_equiv l1 l2 ->
+    stutter_equiv l3 l4 ->
+    stutter_equiv (l1 ++ l3) (l2 ++ l4).
+Proof.
+intros l1 l2 l3 l4 H12 H34.
+transitivity (l2 ++ l3).
+apply stutter_equiv_app_right; assumption.
+apply stutter_equiv_app_left; assumption.
+Qed.
+
+Fixpoint repeat {A} (a: A) (n: nat) : list A :=
+match n with
+| O => nil
+| S n => a :: repeat a n
+end.
+
+Lemma stutter_equiv_repeat {A} :
+  forall (a: A) n,
+    stutter_equiv (a :: nil) (a :: repeat a n).
+Proof.
+intros a n. induction n; simpl; auto.
+Qed.
+
+Lemma repeat_length {A} :
+  forall (a: A) n, length (repeat a n) = n.
+Proof.
+intros a n. induction n; simpl in *; auto.
+Qed.
+
+Lemma In_nth {A} :
+  forall a (l: list A),
+    In a l -> exists n, n < length l /\ forall b, nth n l b = a.
+Proof.
+intros a l H. generalize dependent a. induction l; intros a' H'.
+* destruct H'.
+* destruct H'.
+  + subst a'. exists 0. split; auto.
+  + destruct (IHl a' H) as [n [Hn Hnth]].
+    exists (S n). split; auto.
+Qed.
+
+Lemma repeat_nth {A} :
+  forall (a a0 : A) k n,
+    k < n ->
+    nth k (repeat a n) a0 = a.
+Proof.
+intros a a0 k n H.
+generalize dependent k. revert a. induction n; intros a k H; auto.
+simpl. destruct k; auto.
+Qed.
+
+Lemma stutter_one_inv {A} :
+  forall a (l: list A),
+    stutter_equiv l (a :: nil) ->
+    exists n, l = a :: repeat a n.
+Proof.
+intros a l H. induction l.
+* apply stutter_equiv_nil_left_inv in H. congruence.
+* assert (a0 = a). { apply stutter_equiv_cons_inv in H. assumption. }
+  subst a0. inversion H; subst.
+  + exists 0. apply stutter_equiv_nil_right_inv in H1. subst. reflexivity.
+  + destruct IHl as [n Heq]; trivial.
+    exists (S n). rewrite Heq. reflexivity.
+Qed.
+
+Lemma stutter_two_inv {A} :
+  forall a1 a2 (l: list A),
+    a1 <> a2 ->
+    stutter_equiv l (a1 :: a2 :: nil) ->
+    exists n1 n2, l = a1 :: repeat a1 n1 ++ a2 :: repeat a2 n2.
+Proof.
+intros a1 a2 l Ha Hl. induction l.
+* apply stutter_equiv_nil_left_inv in Hl. congruence.
+* assert (a = a1). { apply stutter_equiv_cons_inv in Hl. assumption. }
+  subst a. destruct l as [| a l].
+  + inversion Hl; subst.
+    - apply stutter_equiv_nil_left_inv in H0. congruence.
+    - congruence.
+  + inversion Hl; subst.
+    - destruct (stutter_one_inv _ _ H0) as [n2 Hn2].
+      exists 0. exists n2. simpl. congruence.
+    - destruct IHl as [n1 [n2 Heq]]; trivial.
+      exists (S n1). exists n2. simpl. congruence.
+    - congruence.
+Qed.
+
+Lemma stutter_equiv_app_left_inv {A} :
+  forall a (l1 l2 l3: list A),
+    stutter_equiv (l1 ++ a :: l2) l3 ->
+    exists l1' l2',
+      l3 = l1' ++ a :: l2'
+      /\ stutter_equiv (l1 ++ a :: nil) (l1' ++ a :: nil)
+      /\ stutter_equiv (a :: l2) (a :: l2').
+Proof.
+intros a l1 l2 l3 H.
+remember (l1 ++ a :: l2) as l1'.
+generalize dependent l2. revert a l1. rename l1' into l1.
+induction H; intros a' l1' l2' Heq.
+* exfalso. destruct l1'; inversion Heq.
+* destruct l1' as [|a1' l1'].
+  - inversion Heq; subst.
+    exists nil. exists l2. simpl. auto.
+  - rewrite <- app_comm_cons in Heq. inversion Heq; subst.
+    destruct (IHstutter_equiv a' l1' l2' eq_refl) as [l1'' [l2'' [? [? ?]]]].
+    subst.
+    exists (a1' :: l1''). exists l2''.
+    repeat rewrite <- app_comm_cons. auto.
+* destruct l1' as [|a1' l1'].
+  - inversion Heq; subst.
+    destruct (IHstutter_equiv a' nil l1 eq_refl) as [l1'' [l2'' [? [? ?]]]].
+    subst. exists l1''. exists l2''. auto.
+  - rewrite <- app_comm_cons in Heq. inversion Heq; subst.
+    destruct (stutter_equiv_cons_left_inv _ _ _ H) as [l2'' H2''].
+    subst.
+    destruct (IHstutter_equiv a' l1' l2' H2) as [l1'' [l0 [? [? ?]]]].
+    exists l1''. exists l0. splits; trivial.
+    { destruct l1'' as [|a1'' l1''].
+      * inversion H0; subst. clear H0.
+        destruct (stutter_one_inv _ _ H1) as [n Hn].
+        rewrite <- app_comm_cons. rewrite Hn.
+        apply stutter_left. symmetry. apply stutter_equiv_repeat.
+      * rewrite <- app_comm_cons in H0. inversion H0; subst.
+        repeat rewrite <- app_comm_cons.
+        rewrite <- app_comm_cons in H1.
+        apply stutter_equiv_cons_right_add_left. trivial.
+    }
+* subst. destruct l1' as [|a1' l1'].
+  - assert (a' = a). { apply stutter_equiv_cons_inv in H. assumption. }
+    subst. exists (a :: nil). exists l2. simpl; auto.
+  - rewrite <- app_comm_cons in H.
+    assert (a1' = a). { apply stutter_equiv_cons_inv in H. assumption. }
+    subst.
+    destruct (IHstutter_equiv a' (a :: l1') l2' eq_refl)
+      as [l1'' [l2'' [? [? ?]]]].
+    { destruct l1'' as [|a1'' l1''].
+      * inversion H0; subst. clear H0. simpl in *.
+        destruct (stutter_one_inv _ _ H1) as [n Hn].
+        exists (a' :: nil). exists l2''.
+        splits; trivial.
+        simpl. rewrite Hn. apply stutter_right.
+        symmetry. apply stutter_equiv_repeat.
+      * rewrite <- app_comm_cons in H0. inversion H0; subst. clear H0.
+        exists (a1'' :: a1'' :: l1''). exists l2''.
+        repeat rewrite <- app_comm_cons. auto.
+    }
+Qed.
+
+Lemma stutter_equiv_app_right_inv {A} :
+  forall a (l1 l2 l3: list A),
+    stutter_equiv l1 (l2 ++ a :: l3) ->
+    exists l2' l3',
+      l1 = l2' ++ a :: l3'
+      /\ stutter_equiv (l2' ++ a :: nil) (l2 ++ a :: nil)
+      /\ stutter_equiv (a :: l3') (a :: l3).
+Proof.
+intros a l1 l2 l3 H.
+symmetry in H.
+destruct (stutter_equiv_app_left_inv _ _ _ _ H) as [l2' [l3' [? [? ?]]]].
+exists l2'. exists l3'. symmetry in H1. symmetry in H2. auto.
+Qed.
+
